add windows proofs

x86/proofs/mldsa_pointwise_acc_l4.ml
@@ -521,3 +521,201 @@ let MLDSA_POINTWISE_ACC_L4_SUBROUTINE_CORRECT = prove
   CONV_TAC TWEAK_CONV THEN
   MATCH_ACCEPT_TAC(ADD_IBT_RULE
     (CONV_RULE TWEAK_CONV MLDSA_POINTWISE_ACC_L4_NOIBT_SUBROUTINE_CORRECT)));;
+
+(* ========================================================================= *)
+(* Windows ABI subroutine form                                               *)
+(* ========================================================================= *)
+
+let mldsa_pointwise_acc_l4_windows_mc = define_from_elf
+   "mldsa_pointwise_acc_l4_windows_mc" "x86/mldsa/mldsa_pointwise_acc_l4.obj";;
+
+let mldsa_pointwise_acc_l4_windows_tmc =
+  define_trimmed "mldsa_pointwise_acc_l4_windows_tmc"
+    mldsa_pointwise_acc_l4_windows_mc;;
+
+let MLDSA_POINTWISE_ACC_L4_WINDOWS_TMC_EXEC =
+  X86_MK_EXEC_RULE mldsa_pointwise_acc_l4_windows_tmc;;
+
+let MLDSA_POINTWISE_ACC_L4_NOIBT_WINDOWS_SUBROUTINE_CORRECT = prove
+ (`!c a b consts x y pc stackpointer returnaddress.
+    aligned 32 c /\
+    aligned 32 a /\
+    aligned 32 b /\
+    aligned 32 consts /\
+    nonoverlapping (word pc,LENGTH mldsa_pointwise_acc_l4_windows_tmc) (c, 1024) /\
+    nonoverlapping (word pc,LENGTH mldsa_pointwise_acc_l4_windows_tmc) (a, 4096) /\
+    nonoverlapping (word pc,LENGTH mldsa_pointwise_acc_l4_windows_tmc) (b, 4096) /\
+    nonoverlapping (word pc,LENGTH mldsa_pointwise_acc_l4_windows_tmc) (consts, 64) /\
+    nonoverlapping (c, 1024) (a, 4096) /\
+    nonoverlapping (c, 1024) (b, 4096) /\
+    nonoverlapping (c, 1024) (consts, 64) /\
+    nonoverlapping (a, 4096) (b, 4096) /\
+    nonoverlapping (a, 4096) (consts, 64) /\
+    nonoverlapping (b, 4096) (consts, 64) /\
+    nonoverlapping (word_sub stackpointer (word 176),184) (c, 1024) /\
+    nonoverlapping (word_sub stackpointer (word 176),184) (a, 4096) /\
+    nonoverlapping (word_sub stackpointer (word 176),184) (b, 4096) /\
+    nonoverlapping (word_sub stackpointer (word 176),184) (consts, 64) /\
+    nonoverlapping (word pc,LENGTH mldsa_pointwise_acc_l4_windows_tmc)
+                   (word_sub stackpointer (word 176),176)
+    ==> ensures x86
+          (\s. bytes_loaded s (word pc) mldsa_pointwise_acc_l4_windows_tmc /\
+              read RIP s = word pc /\
+              read RSP s = stackpointer /\
+              read (memory :> bytes64 stackpointer) s = returnaddress /\
+              WINDOWS_C_ARGUMENTS [c; a; b; consts] s /\
+              wordlist_from_memory(consts,16) s =
+                MAP (iword: int -> 32 word) mldsa_pointwise_acc_l4_consts /\
+              (!i. i < 1024 ==> abs(ival(x i)) <= &8380416) /\
+              (!i. i < 1024 ==> abs(ival(y i)) <= &75423752) /\
+              (!i. i < 1024 ==>
+                read(memory :> bytes32(word_add a (word(4 * i)))) s = x i) /\
+              (!i. i < 1024 ==>
+                read(memory :> bytes32(word_add b (word(4 * i)))) s = y i))
+          (\s. read RIP s = returnaddress /\
+              read RSP s = word_add stackpointer (word 8) /\
+              (!i. i < 256 ==>
+                let zi = read(memory :> bytes32(word_add c (word(4 * i)))) s in
+                (ival zi == mldsa_pointwise_acc_l4 (ival o x) (ival o y) i)
+                  (mod &8380417) /\
+                abs(ival zi) <= &8380416))
+          (MAYCHANGE [RSP] ,,
+           WINDOWS_MAYCHANGE_REGS_AND_FLAGS_PERMITTED_BY_ABI ,,
+           MAYCHANGE [memory :> bytes(word_sub stackpointer (word 176),176)] ,,
+           MAYCHANGE [memory :> bytes(c, 1024)])`,
+  let TWEAK_CONV = ONCE_DEPTH_CONV WORDLIST_FROM_MEMORY_CONV in
+  CONV_TAC TWEAK_CONV THEN
+  REPLICATE_TAC 7 GEN_TAC THEN
+  WORD_FORALL_OFFSET_TAC 176 THEN REPEAT GEN_TAC THEN
+
+  REWRITE_TAC[fst MLDSA_POINTWISE_ACC_L4_WINDOWS_TMC_EXEC] THEN
+  REPEAT STRIP_TAC THEN REWRITE_TAC[WINDOWS_C_ARGUMENTS] THEN
+  REWRITE_TAC[WINDOWS_MAYCHANGE_REGS_AND_FLAGS_PERMITTED_BY_ABI] THEN
+
+  ENSURES_PRESERVED_TAC "rdi_init" `RDI` THEN
+  ENSURES_PRESERVED_TAC "rsi_init" `RSI` THEN
+  ENSURES_PRESERVED_TAC "init_xmm6" `ZMM6 :> bottomhalf :> bottomhalf` THEN
+  ENSURES_PRESERVED_TAC "init_xmm7" `ZMM7 :> bottomhalf :> bottomhalf` THEN
+  ENSURES_PRESERVED_TAC "init_xmm8" `ZMM8 :> bottomhalf :> bottomhalf` THEN
+  ENSURES_PRESERVED_TAC "init_xmm9" `ZMM9 :> bottomhalf :> bottomhalf` THEN
+  ENSURES_PRESERVED_TAC "init_xmm10" `ZMM10 :> bottomhalf :> bottomhalf` THEN
+  ENSURES_PRESERVED_TAC "init_xmm11" `ZMM11 :> bottomhalf :> bottomhalf` THEN
+  ENSURES_PRESERVED_TAC "init_xmm12" `ZMM12 :> bottomhalf :> bottomhalf` THEN
+  ENSURES_PRESERVED_TAC "init_xmm13" `ZMM13 :> bottomhalf :> bottomhalf` THEN
+  ENSURES_PRESERVED_TAC "init_xmm14" `ZMM14 :> bottomhalf :> bottomhalf` THEN
+  ENSURES_PRESERVED_TAC "init_xmm15" `ZMM15 :> bottomhalf :> bottomhalf` THEN
+
+  REWRITE_TAC[READ_ZMM_BOTTOM_QUARTER'] THEN
+  REWRITE_TAC(map GSYM
+    [YMM6;YMM7;YMM8;YMM9;YMM10;YMM11;YMM12;YMM13;YMM14;YMM15]) THEN
+
+  GHOST_INTRO_TAC `init_ymm6:int256` `read YMM6` THEN
+  GHOST_INTRO_TAC `init_ymm7:int256` `read YMM7` THEN
+  GHOST_INTRO_TAC `init_ymm8:int256` `read YMM8` THEN
+  GHOST_INTRO_TAC `init_ymm9:int256` `read YMM9` THEN
+  GHOST_INTRO_TAC `init_ymm10:int256` `read YMM10` THEN
+  GHOST_INTRO_TAC `init_ymm11:int256` `read YMM11` THEN
+  GHOST_INTRO_TAC `init_ymm12:int256` `read YMM12` THEN
+  GHOST_INTRO_TAC `init_ymm13:int256` `read YMM13` THEN
+  GHOST_INTRO_TAC `init_ymm14:int256` `read YMM14` THEN
+  GHOST_INTRO_TAC `init_ymm15:int256` `read YMM15` THEN
+
+  GLOBALIZE_PRECONDITION_TAC THEN
+  REPEAT(FIRST_X_ASSUM(SUBST1_TAC o SYM)) THEN
+
+  (* Execute Windows prologue: 17 instructions *)
+  ENSURES_INIT_TAC "s0" THEN
+  X86_STEPS_TAC MLDSA_POINTWISE_ACC_L4_WINDOWS_TMC_EXEC (1--17) THEN
+
+  (* Reuse the Unix proof for the core pointwise computation *)
+  MP_TAC(SPECL
+    [`c:int64`; `a:int64`; `b:int64`; `consts:int64`;
+     `x:num->int32`; `y:num->int32`; `pc + 98`]
+    (CONV_RULE(ONCE_DEPTH_CONV(REWRITE_CONV
+       [MAYCHANGE_REGS_AND_FLAGS_PERMITTED_BY_ABI; SOME_FLAGS]))
+      (CONV_RULE TWEAK_CONV MLDSA_POINTWISE_ACC_L4_CORRECT))) THEN
+  ASM_REWRITE_TAC[C_ARGUMENTS] THEN
+  ANTS_TAC THENL [NONOVERLAPPING_TAC; ALL_TAC] THEN
+
+  (* Execute core computation as one big step *)
+  X86_BIGSTEP_TAC MLDSA_POINTWISE_ACC_L4_WINDOWS_TMC_EXEC "s18" THENL
+   [FIRST_ASSUM(MATCH_ACCEPT_TAC o MATCH_MP
+     (BYTES_LOADED_SUBPROGRAM_RULE mldsa_pointwise_acc_l4_windows_tmc
+     (REWRITE_RULE[BUTLAST_CLAUSES]
+      (AP_TERM `BUTLAST:byte list->byte list` mldsa_pointwise_acc_l4_tmc))
+     98));
+    RULE_ASSUM_TAC(CONV_RULE(TRY_CONV RIP_PLUS_CONV))] THEN
+
+  (* Capture final YMM states before epilogue *)
+  MAP_EVERY ABBREV_TAC
+   [`ymm6_epilog = read YMM6 s18`;
+    `ymm7_epilog = read YMM7 s18`;
+    `ymm8_epilog = read YMM8 s18`;
+    `ymm9_epilog = read YMM9 s18`;
+    `ymm10_epilog = read YMM10 s18`;
+    `ymm11_epilog = read YMM11 s18`;
+    `ymm12_epilog = read YMM12 s18`;
+    `ymm13_epilog = read YMM13 s18`;
+    `ymm14_epilog = read YMM14 s18`;
+    `ymm15_epilog = read YMM15 s18`] THEN
+
+  (* Execute Windows epilogue: 14 instructions including RET *)
+  X86_STEPS_TAC MLDSA_POINTWISE_ACC_L4_WINDOWS_TMC_EXEC (19--32) THEN
+
+  RULE_ASSUM_TAC(REWRITE_RULE[MAYCHANGE_ZMM_QUARTER]) THEN
+  RULE_ASSUM_TAC(REWRITE_RULE[MAYCHANGE_YMM_SSE_QUARTER]) THEN
+
+  ENSURES_FINAL_STATE_TAC THEN ASM_REWRITE_TAC[] THEN
+  REPEAT CONJ_TAC THEN CONV_TAC WORD_BLAST);;
+
+let MLDSA_POINTWISE_ACC_L4_WINDOWS_SUBROUTINE_CORRECT = prove
+ (`!c a b consts x y pc stackpointer returnaddress.
+    aligned 32 c /\
+    aligned 32 a /\
+    aligned 32 b /\
+    aligned 32 consts /\
+    nonoverlapping (word pc,LENGTH mldsa_pointwise_acc_l4_windows_mc) (c, 1024) /\
+    nonoverlapping (word pc,LENGTH mldsa_pointwise_acc_l4_windows_mc) (a, 4096) /\
+    nonoverlapping (word pc,LENGTH mldsa_pointwise_acc_l4_windows_mc) (b, 4096) /\
+    nonoverlapping (word pc,LENGTH mldsa_pointwise_acc_l4_windows_mc) (consts, 64) /\
+    nonoverlapping (c, 1024) (a, 4096) /\
+    nonoverlapping (c, 1024) (b, 4096) /\
+    nonoverlapping (c, 1024) (consts, 64) /\
+    nonoverlapping (a, 4096) (b, 4096) /\
+    nonoverlapping (a, 4096) (consts, 64) /\
+    nonoverlapping (b, 4096) (consts, 64) /\
+    nonoverlapping (word_sub stackpointer (word 176),184) (c, 1024) /\
+    nonoverlapping (word_sub stackpointer (word 176),184) (a, 4096) /\
+    nonoverlapping (word_sub stackpointer (word 176),184) (b, 4096) /\
+    nonoverlapping (word_sub stackpointer (word 176),184) (consts, 64) /\
+    nonoverlapping (word pc,LENGTH mldsa_pointwise_acc_l4_windows_mc)
+                   (word_sub stackpointer (word 176),176)
+    ==> ensures x86
+          (\s. bytes_loaded s (word pc) mldsa_pointwise_acc_l4_windows_mc /\
+              read RIP s = word pc /\
+              read RSP s = stackpointer /\
+              read (memory :> bytes64 stackpointer) s = returnaddress /\
+              WINDOWS_C_ARGUMENTS [c; a; b; consts] s /\
+              wordlist_from_memory(consts,16) s =
+                MAP (iword: int -> 32 word) mldsa_pointwise_acc_l4_consts /\
+              (!i. i < 1024 ==> abs(ival(x i)) <= &8380416) /\
+              (!i. i < 1024 ==> abs(ival(y i)) <= &75423752) /\
+              (!i. i < 1024 ==>
+                read(memory :> bytes32(word_add a (word(4 * i)))) s = x i) /\
+              (!i. i < 1024 ==>
+                read(memory :> bytes32(word_add b (word(4 * i)))) s = y i))
+          (\s. read RIP s = returnaddress /\
+              read RSP s = word_add stackpointer (word 8) /\
+              (!i. i < 256 ==>
+                let zi = read(memory :> bytes32(word_add c (word(4 * i)))) s in
+                (ival zi == mldsa_pointwise_acc_l4 (ival o x) (ival o y) i)
+                  (mod &8380417) /\
+                abs(ival zi) <= &8380416))
+          (MAYCHANGE [RSP] ,,
+           WINDOWS_MAYCHANGE_REGS_AND_FLAGS_PERMITTED_BY_ABI ,,
+           MAYCHANGE [memory :> bytes(word_sub stackpointer (word 176),176)] ,,
+           MAYCHANGE [memory :> bytes(c, 1024)])`,
+  let TWEAK_CONV = ONCE_DEPTH_CONV WORDLIST_FROM_MEMORY_CONV in
+  CONV_TAC TWEAK_CONV THEN
+  MATCH_ACCEPT_TAC(ADD_IBT_RULE
+    (CONV_RULE TWEAK_CONV MLDSA_POINTWISE_ACC_L4_NOIBT_WINDOWS_SUBROUTINE_CORRECT)));;
